proof/DDC/Language/SystemF.v
@@ -1,0 +1,42 @@
+(* System-F.
+   Like STLC, but with type abstraction and application. *)
+
+(* Kinds and kind environemnts. *)
+Require Export DDC.Language.SystemF.Ki.
+
+(* Types, well formed and closed, lifting and substitution lemmas. *)
+Require Export DDC.Language.SystemF.Ty.
+
+(* Type environments, lifting and substitution lemmas. *)
+Require Export DDC.Language.SystemF.TyEnv.
+
+(* Expressions, normal forms, lifting and substitution. *)
+Require Export DDC.Language.SystemF.Exp.
+
+(* Kinds of types, weakening the kind environment. *)
+Require Export DDC.Language.SystemF.KiJudge.
+
+(* Substitution of types in types preserves kinding. *)
+Require Export DDC.Language.SystemF.SubstTypeType.
+
+(* Type Judgement. *)
+Require Export DDC.Language.SystemF.TyJudge.
+
+(* Substitution of types in expressions preserves typing. *)
+Require Export DDC.Language.SystemF.SubstTypeExp.
+
+(* Substitution of expressions in expressions preserves typing. *)
+Require Export DDC.Language.SystemF.SubstExpExp.
+
+(* Small step evaluation. *)
+Require Export DDC.Language.SystemF.Step.
+
+(* A well typed expression is either a value, or can take a step. *)
+Require Export DDC.Language.SystemF.Progress.
+
+(* When an expression takes a step the results has the same type. *)
+Require Export DDC.Language.SystemF.Preservation.
+
+(* Big step evaluation, and conversion to small steps. *)
+Require Export DDC.Language.SystemF.Eval.
+
