proof/DDC/Language/SystemF/Eval.v
@@ -1,13 +1,14 @@
 
-Require Export SubstExpExp.
-Require Export SubstTypeExp.
-Require Import Preservation.
-Require Import TyJudge.
-Require Export EsJudge.
-Require Export Exp.
+Require Import DDC.Language.SystemF.Preservation.
+Require Export DDC.Language.SystemF.Step.
+Require Export DDC.Language.SystemF.SubstExpExp.
+Require Export DDC.Language.SystemF.SubstTypeExp.
+Require Import DDC.Language.SystemF.TyJudge.
+Require Export DDC.Language.SystemF.Exp.
 
 
-(* Big Step Evaluation **********************************************
+(********************************************************************)
+(* Big Step Evaluation
    This is also called 'Natural Semantics'.
    It provides a relation between the expression to be reduced 
    and its final value. 
@@ -15,8 +16,8 @@ Require Export Exp.
 Inductive EVAL : exp -> exp -> Prop :=
  | EVDone
    :  forall v2
-   ,  whnfX  v2
-   -> EVAL   v2 v2
+   ,  wnfX v2
+   -> EVAL v2 v2
 
  | EVLAMAPP
    : forall x1 x12 t2 v3
@@ -31,28 +32,26 @@ Inductive EVAL : exp -> exp -> Prop :=
 Hint Constructors EVAL.
 
 
-(* A terminating big-step evaluation always produces a whnf.
+(* A terminating big-step evaluation always produces a wnf.
    The fact that the evaluation terminated is implied by the fact
    that we have a finite proof of EVAL to pass to this lemma. 
  *)
-Lemma eval_produces_whnfX
+Lemma eval_produces_wnfX
  :  forall x1 v1
  ,  EVAL   x1 v1
- -> whnfX  v1.
+ -> wnfX  v1.
 Proof.
  intros. induction H; eauto.
 Qed.
-Hint Resolve eval_produces_whnfX.
+Hint Resolve eval_produces_wnfX.
 
 
-(* Big to Small steps ***********************************************
-   Convert a big-step evaluation into a list of individual
-   machine steps.
- *)
+(********************************************************************)
+(* Convert a big-step evaluation into a list of small steps. *)
 Lemma steps_of_eval
  :  forall x1 t1 x2
- ,  TYPE Empty Empty x1 t1
- -> EVAL x1 x2
+ ,  TYPE nil nil x1 t1
+ -> EVAL  x1 x2
  -> STEPS x1 x2.
 Proof.
  intros x1 t1 v2 HT HE. gen t1.
@@ -68,8 +67,6 @@ Proof.
   lets T1: preservation_steps H3 E1. inverts keep T1.
   lets T2: subst_type_value H4 H5.
    simpl in T2.
-    assert (substTE 0 t2 (liftTE 0 Empty) = Empty). auto.
-    rewrite H in T2. clear H.
   lets E2: IHHE2 T2.
   eapply ESAppend.
    apply steps_APP1. eauto.
@@ -96,11 +93,11 @@ Proof.
 Qed.
 
 
-(* Small to Big steps ***********************************************
-   Convert a list of individual machine steps to a big-step
-   evaluation. The main part of this is the expansion lemma, which 
-   we use to build up the overall big-step evaluation one small-step
-   at a time. The other lemmas are used to feed it small-steps.
+(********************************************************************)
+(* Convert a list of small steps to a big-step evaluation. The main
+   part of this is the expansion lemma, which we use to build up the
+   overall big-step evaluation one small-step at a time. The other
+  lemmas are used to feed it small-steps.
  *)
 
 (* Given an existing big-step evalution, we can produce a new one
@@ -151,7 +148,7 @@ Qed.
 (* Convert a list of small steps to a big-step evaluation. *)
 Lemma eval_of_stepsl
  :  forall x1 t1 v2
- ,  TYPE Empty Empty x1 t1
+ ,  TYPE nil nil x1 t1
  -> STEPSL x1 v2 -> value v2
  -> EVAL   x1 v2.
 Proof.
@@ -176,7 +173,7 @@ Qed.
  *)
 Lemma eval_of_steps
  :  forall x1 t1 v2
- ,  TYPE Empty Empty x1 t1
+ ,  TYPE nil nil x1 t1
  -> STEPS x1 v2 -> value v2
  -> EVAL  x1 v2.
 Proof.
