proof/DDC/Language/SystemF/Ki.v
@@ -1,0 +1,14 @@
+
+Require Export DDC.Base.
+
+
+(* Kind expressions *)
+Inductive ki : Type :=
+ | KStar   : ki.
+
+
+(* Kind environments. *)
+Definition kienv := list ki.
+Hint Unfold kienv.
+
+
