proof/DDC/Language/SystemF/KiJudge.v
@@ -1,0 +1,93 @@
+
+Require Export DDC.Language.SystemF.Ty.
+Require Export DDC.Language.SystemF.Ki.
+
+
+(* Kind judgement assigns a kind to a type.
+
+   With plain SystemF (not SystemF2) we only have value types.
+   We could have made this a 2-place relation and omitted the 
+   KStar return kind, but doing it this way makes the form of the 
+   judgement more similar to the SystemF2 case. 
+ *)
+Inductive KIND : kienv -> ty -> ki -> Prop :=
+ | KICon 
+   :  forall ke c
+   ,  KIND ke (TCon c) KStar
+
+ | KIVar
+   :  forall ke i k
+   ,  get  i ke = Some k
+   -> KIND ke (TVar i) k
+
+ | KIForall
+   :  forall ke t
+   ,  KIND (ke :> KStar) t           KStar
+   -> KIND ke            (TForall t) KStar
+
+ | KIFun 
+   :  forall ke t1 t2
+   ,  KIND ke t1 KStar
+   -> KIND ke t2 KStar
+   -> KIND ke (TFun t1 t2) KStar.
+
+Hint Constructors KIND.
+
+
+(********************************************************************)
+(* A well kinded type is well formed. *)
+Lemma kind_wfT
+ :  forall ke t k
+ ,  KIND ke t k
+ -> wfT  ke t.
+Proof.
+ intros. gen ke k.
+ induction t; intros; inverts H; simpl; eauto.
+Qed.
+
+
+(* If a type is well kinded in an empty environment,
+   then that type is closed. *)
+Lemma kind_empty_is_closed
+ :  forall t k
+ ,  KIND nil t k 
+ -> closedT t.
+Proof.
+ intros. unfold closedT. eapply kind_wfT. eauto.
+Qed.
+
+
+(* We can insert a new type into the environment at an arbitray point
+   provided we lift existing references to types higher than this
+   point across the new one. *)
+Lemma liftTT_insert
+ :  forall ke ix t k1 k2
+ ,  KIND ke t k1
+ -> KIND (insert ix k2 ke) (liftTT ix t) k1.
+Proof.
+ intros. gen ix ke k1.
+ induction t; intros; simpl; inverts H; eauto.
+
+ Case "TVar".
+  lift_cases; intros; auto.
+
+ Case "TForall".
+  apply KIForall.
+  rewrite insert_rewind.
+  apply IHt. auto.
+Qed.
+
+
+(* Weakening the kind environment by pushing a new type onto the
+   stack *)
+Lemma liftTT_weaken
+ :  forall ke t k1 k2
+ ,  KIND  ke         t           k1
+ -> KIND (ke :> k2) (liftTT 0 t) k1.
+Proof.
+ intros.
+ assert (ke :> k2 = insert 0 k2 ke). simpl.
+   destruct ke; auto.
+ rewrite H0. apply liftTT_insert. auto.
+Qed.
+
