proof/Main.v
@@ -1,4 +1,9 @@
 (* Top level module imports everything so that we have a
    nice make target to build the proofs. *)
 Require Import DDC.Base.
+
+(* Simply Typed Lambda Calculus (STLC) *).
 Require Import DDC.Language.Simple.
+
+(* System-F. Like STLC, but with type abstraction and application. *)
+Require Import DDC.Language.SystemF.
